cappy: subtyping translation proof

Cappy/Translation/Subtyping.lean
@@ -1,4 +1,51 @@
 import Cappy.Translation.Subcapturing
+import Cappy.TypeSystem
+import Capless.Subtyping
 namespace Cappy
+
+def CType.interp_monotonic.motive_1
+  (Γ : Context n m)
+  (T1 T2 : CType n m)
+  (_ : CSubtyp Γ T1 T2) : Prop :=
+  ∀ {k} {Δ : Capless.Context n m k} {ρ} (_ : Context.Interp Γ ⟨Δ, ρ⟩)
+    {D1 Q1} (_ : CType.Interp ρ Γ T1 D1 Q1),
+  ∃ D2 Q2,
+    CType.Interp ρ Γ T2 D2 Q2 ∧
+    (Δ ⊢ Q1 <: Q2)
+
+def CType.interp_monotonic.motive_2
+  (Γ : Context n m)
+  (S1 S2 : SType n m)
+  (_ : SSubtyp Γ S1 S2) : Prop :=
+  ∀ {k} {Δ : Capless.Context n m k} {ρ} (_ : Context.Interp Γ ⟨Δ, ρ⟩)
+    {C D1 Q1} (_ : CType.Interp ρ Γ (S1^C) D1 Q1),
+  ∃ D2 Q2,
+    CType.Interp ρ Γ (S2^C) D2 Q2 ∧
+    (Δ ⊢ Q1 <: Q2)
+
+
+theorem CType.interp_monotonic
+  (hg : Context.Interp Γ ⟨Δ, ρ⟩)
+  (hsub : CSubtyp Γ T1 T2)
+  (hi : CType.Interp ρ Γ T1 D1 Q1) :
+  ∃ D2 Q2,
+    CType.Interp ρ Γ T2 D2 Q2 ∧
+    (Δ ⊢ Q1 <: Q2) := by
+  apply CSubtyp.rec
+    (motive_1 := CType.interp_monotonic.motive_1)
+    (motive_2 := CType.interp_monotonic.motive_2)
+    (t := hsub)
+    (D1 := D1)
+  all_goals try assumption
+  case capt =>
+    repeat intro
+    sorry
+  case top => sorry
+  case refl => sorry
+  case trans => sorry
+  case tvar => sorry
+  case boxed => sorry
+  case arrow => sorry
+  case tarrow => sorry
 
 end Cappy
